feat: coercionを使用しないように変更

src/Michio Suzuki (1982) Group Theory I/main.v
@@ -8,7 +8,7 @@ Require Import Coq.Logic.Classical_Prop.
 (* Definition 1.1. *)
 Structure group : Type := make_group
 {
-  group_carrier :> Set;
+  group_carrier : Set;
   group_inhab : inhabited group_carrier;
   group_mul : group_carrier -> group_carrier -> group_carrier;
   group_mul_assoc : forall a b c : group_carrier, group_mul (group_mul a b) c = group_mul a (group_mul b c);
@@ -17,19 +17,19 @@ Structure group : Type := make_group
 }.
 
 (* Definition 1.3. *)
-Definition is_group_one (G : group) (e : G) :=
-  forall g : G, group_mul G g e = g /\ group_mul G e g = g.
+Definition is_group_one (G : group) (e : group_carrier G) :=
+  forall g : group_carrier G, group_mul G g e = g /\ group_mul G e g = g.
 
 (* Theorem 1.2.(ii)' *)
 Theorem group_one_exists_unique (G : group) :
-  exists! group_one : G, is_group_one G group_one.
+  exists! group_one : group_carrier G, is_group_one G group_one.
 Proof.
   destruct (group_inhab G) as [a].
   destruct (group_eq_l G a a) as [e Hae_eq_a].
   destruct (group_eq_r G a a) as [e' He'a_eq_a].
   exists e.
 
-  assert (forall g : G, group_mul G g e = g) as He_oner.
+  assert (forall g : group_carrier G, group_mul G g e = g) as He_oner.
   + move=> g.
     destruct (group_eq_l G a g) as [u Hau_eq_g].
     destruct (group_eq_r G a g) as [v Hva_eq_g].
@@ -38,7 +38,7 @@ Proof.
     rewrite Hae_eq_a.
     by [].
 
-  assert (forall g : G, group_mul G e' g = g) as He'_onel.
+  assert (forall g : group_carrier G, group_mul G e' g = g) as He'_onel.
   + move=> g.
     destruct (group_eq_l G a g) as [u Hau_eq_g].
     destruct (group_eq_r G a g) as [v Hva_eq_g].
@@ -66,7 +66,7 @@ Proof.
     by [].
 Qed.
 
-Definition group_one (G : group) : G.
+Definition group_one (G : group) : group_carrier G.
   destruct (constructive_definite_description (is_group_one G) (group_one_exists_unique G)) as [group_one H].
   exact group_one.
 Defined.
@@ -80,12 +80,12 @@ Proof.
   exact He'.
 Qed.
 
-Definition are_mut_inv (G : group) (a a' : G) :=
+Definition are_mut_inv (G : group) (a a' : group_carrier G) :=
   group_mul G a a' = group_one G /\ group_mul G a' a = group_one G.
 
 (* Theorem 1.2.(ii)'' *)
-Theorem group_inv_ex_uni (G : group) (a : G) :
-  exists! a' : G, are_mut_inv G a a'.
+Theorem group_inv_ex_uni (G : group) (a : group_carrier G) :
+  exists! a' : group_carrier G, are_mut_inv G a a'.
 Proof.
   destruct (group_eq_l G a (group_one G)) as [a' Haa'_eq_one].
   destruct (group_eq_r G a (group_one G)) as [a'' Ha''a_eq_one].
@@ -114,13 +114,13 @@ Proof.
     by [].
 Qed.
 
-Definition group_inv (G : group) : G -> G.
+Definition group_inv (G : group) : group_carrier G -> group_carrier G.
   move=> a.
   destruct (constructive_definite_description (are_mut_inv G a) (group_inv_ex_uni G a)) as [a' H].
   exact a'.
 Defined.
 
-Theorem group_inv_is_group_inv (G : group) (a : G) : are_mut_inv G a (group_inv G a).
+Theorem group_inv_is_group_inv (G : group) (a : group_carrier G) : are_mut_inv G a (group_inv G a).
 Proof.
   remember (group_inv G a) as a' eqn: H.
   unfold group_inv in H.
@@ -131,7 +131,7 @@ Qed.
 
 (* Theorem 1.2.(iii).1 *)
 Theorem group_eq_l_ex_uni (G : group) :
-  forall a b x : G, group_mul G a x = b -> x = group_mul G (group_inv G a) b.
+  forall a b x : group_carrier G, group_mul G a x = b -> x = group_mul G (group_inv G a) b.
 Proof.
   move=> a b x Hax_eq_b.
   rewrite -Hax_eq_b.
@@ -143,7 +143,7 @@ Qed.
 
 (* Theorem 1.2.(iii).2 *)
 Theorem group_eq_r_ex_uni (G : group) :
-  forall a b y : G, group_mul G y a = b -> y = group_mul G b (group_inv G a).
+  forall a b y : group_carrier G, group_mul G y a = b -> y = group_mul G b (group_inv G a).
 Proof.
   move=> a b y Hya_eq_b.
   rewrite -Hya_eq_b.
@@ -156,7 +156,7 @@ Qed.
 (* Corollary_p4_l7 *)
 Structure group' : Type := make_group'
 {
-  group'_carrier :> Set;
+  group'_carrier : Set;
   group'_one : group'_carrier;
   group'_inv : group'_carrier -> group'_carrier;
   group'_mul : group'_carrier -> group'_carrier -> group'_carrier;
@@ -167,10 +167,9 @@ Structure group' : Type := make_group'
   group'_mul_inv : forall a : group'_carrier, group'_mul a (group'_inv a) = group'_one;
 }.
 
-Definition group_to_group' : group -> group'.
-  move=> G.
-  exact (make_group'
-    G
+Definition group_to_group' : group -> group'
+  := fun G => (make_group'
+    (group_carrier G)
     (group_one G)
     (group_inv G)
     (group_mul G)
@@ -179,11 +178,10 @@ Definition group_to_group' : group -> group'.
     (fun a => proj1 (group_one_is_group_one G a))
     (fun a => proj2 (group_inv_is_group_inv G a))
     (fun a => proj1 (group_inv_is_group_inv G a))
-   ).
-Qed.
+  ).
 
 Theorem group'_to_group_sub_r (G' : group') :
-  forall a b : G', exists x : G', group'_mul G' a x = b.
+  forall a b : group'_carrier G', exists x : group'_carrier G', group'_mul G' a x = b.
 Proof.
   move=> a b.
   exists (group'_mul G' (group'_inv G' a) b).
@@ -194,7 +192,7 @@ Proof.
 Qed.
 
 Theorem group'_to_group_sub_l (G' : group') :
-  forall a b : G', exists y : G', group'_mul G' y a = b.
+  forall a b : group'_carrier G', exists y : group'_carrier G', group'_mul G' y a = b.
 Proof.
   move=> a b.
   exists (group'_mul G' b (group'_inv G' a)).
@@ -204,21 +202,19 @@ Proof.
   reflexivity.
 Qed.
 
-Definition group'_to_group : group' -> group.
-  move=> G'.
-  exact (make_group
-    G'
+Definition group'_to_group : group' -> group
+  := fun G' => (make_group
+    (group'_carrier G')
     (inhabits (group'_one G'))
     (group'_mul G')
     (group'_mul_assoc G')
     (group'_to_group_sub_r G')
     (group'_to_group_sub_l G')
   ).
-Qed.
 
 (* Theorem 1.4.1 *)
 Theorem inv_inv (G : group) :
-  forall a : G, group_inv G (group_inv G a) = a.
+  forall a : group_carrier G, group_inv G (group_inv G a) = a.
 Proof.
   move=> a.
 
@@ -239,7 +235,7 @@ Qed.
 
 (* Theorem 1.4.2 *)
 Theorem group_mul_inv_rev (G : group) :
-  forall a b : G, group_inv G (group_mul G a b) = group_mul G (group_inv G b) (group_inv G a).
+  forall a b : group_carrier G, group_inv G (group_mul G a b) = group_mul G (group_inv G b) (group_inv G a).
 Proof.
   move=> a b.
 
@@ -271,10 +267,10 @@ Definition subset (S : Set) := S -> Prop.
 
 Structure subgroup (G : group) : Type := make_subgroup
 {
-  subgroup_carrier :> subset G;
+  subgroup_carrier : subset (group_carrier G);
   subgroup_inhab : inhabited (sig subgroup_carrier);
-  subgroup_mul_mem : forall a b : G, subgroup_carrier a -> subgroup_carrier b -> subgroup_carrier (group_mul G a b);
-  subgroup_inv_mem : forall a : G, subgroup_carrier a -> subgroup_carrier (group_inv G a);
+  subgroup_mul_mem : forall a b : group_carrier  G, subgroup_carrier a -> subgroup_carrier b -> subgroup_carrier (group_mul G a b);
+  subgroup_inv_mem : forall a : group_carrier G, subgroup_carrier a -> subgroup_carrier (group_inv G a);
 }.
 
 (* 2.2.(a) *)
@@ -291,7 +287,7 @@ Proof.
 Qed.
 
 Definition subgroup_incl (G : group) (H : subgroup G) :
-  (sig (subgroup_carrier G H)) -> G
+  (sig (subgroup_carrier G H)) -> group_carrier G
   := fun p => let 'exist x Hx := p in x.
 
 Theorem subgroup_incl_is_injective (G : group) (H : subgroup G) :
